clean up p256adx

src/Arithmetic/P256ADX.v
@@ -13,6 +13,7 @@ Definition p3 :=   0xffffffff00000001%Z.
 
 Definition n : nat := 4.
 Definition bound (_ : nat) : positive := Z.to_pos (2^64).
+Local Notation eval := (eval bound).
 
 Definition two_steps_of_p256_montgomery_reduction xs :=
   let x := hd 0 xs in
@@ -21,13 +22,86 @@ Definition two_steps_of_p256_montgomery_reduction xs :=
   let (x', c) := Z.add_with_get_carry_full (2^64) 0 y x't in
   product_scan_ bound (tl (tl xs)) ([(2^32, x'); (p3, x); (p3, x')] ++ repeat (0,0) (length xs - 5)) h c 0.
 
+Definition p256_mul' x y :=
+  dlet xlo := firstn 2 x in
+  dlet xhi := skipn 2 x in
+  dlet a := mul bound (firstn 2 x) y in
+  dlet a := two_steps_of_p256_montgomery_reduction a in
+  dlet a := add_mul bound a xhi y in
+  dlet a := two_steps_of_p256_montgomery_reduction a in
+  dlet a := condsub bound a (encode bound 4 p256) in
+  firstn 4 a.
+
+Local Notation nth i l d := (nth_default d l i).
+Definition sqr4 xs : list Z :=
+  let x0 := nth 0 xs 0 in let x1 := nth 1 xs 0 in let x2 := nth 2 xs 0 in let x3 := nth 3 xs 0 in
+  dlet acc := product_scan_ bound [] [(0,0); (0,0); (0, 0); (x1, x2)] 0 0 0 in
+  dlet acc := product_scan_ bound acc [(0, 0); (x0, x1); (x0, x2); (x0, x3); (x1, x3); (x2, x3)] 0 0 0 in
+  dlet acc := add_ bound 0 acc acc in
+  dlet acc := fst (add bound 0 acc (diagonal (2^64) [(x0,x0); (x1, x1); (x2, x2); (x3, x3)]))
+  in acc.
+
+Definition p256_sqr' a :=
+  dlet a := sqr4 a in
+  dlet a := two_steps_of_p256_montgomery_reduction a in
+  dlet a := two_steps_of_p256_montgomery_reduction a in
+  dlet a := condsub bound a (encode bound 4 p256) in
+  dlet a := firstn 4 a in
+  a.
+
+(* Versions with bounds-checking assertions *)
+
+Definition p256_mul x y :=
+  if negb (2 <=? Z.of_nat (Datatypes.length x)) then nil else
+  if negb ((0 <=? eval x) && (eval x <? 2^256)) then nil else
+  if negb ((0 <=? eval y) && (eval y <? 2^256)) then nil else
+  dlet xlo := firstn 2 x in
+  dlet xhi := skipn 2 x in
+  if negb ((0 <=? eval xlo) && (eval xlo <? 2^128)) then nil else
+  dlet a := mul bound (firstn 2 x) y in
+  if negb ((0 <=? hd 0 a) && (hd 0 a <? 2 ^ 64)) then nil else
+  if negb ((0 <=? hd 0 (tl a)) && (hd 0 (tl a) <? 2 ^ 64)) then nil else
+  dlet a := two_steps_of_p256_montgomery_reduction a in
+  if negb ((0 <=? eval xhi) && (eval xhi <? 2^128)) then nil else
+  dlet a := add_mul bound a xhi y in
+  if negb ((0 <=? hd 0 a) && (hd 0 a <? 2 ^ 64)) then nil else
+  if negb ((0 <=? hd 0 (tl a)) && (hd 0 (tl a) <? 2 ^ 64)) then nil else
+  dlet a := two_steps_of_p256_montgomery_reduction a in
+  if negb (eval a <? (weight bound (Nat.max (Datatypes.length a) (Datatypes.length (encode bound 4 p256))))) then nil else
+  dlet a := condsub bound a (encode bound 4 p256) in
+  if negb (4 <=? Z.of_nat (Datatypes.length a)) then nil else
+  if negb (isbounded bound a) then nil else
+  firstn 4 a.
+
+Lemma p256_mul'_correct x y : p256_mul x y <> nil -> p256_mul' x y = p256_mul x y.
+Proof. cbv [p256_mul p256_mul' Let_In]; break_match; congruence. Qed.
+
+Definition p256_sqr a :=
+  if negb (4 =? Z.of_nat (Datatypes.length a)) then nil else
+  dlet a := sqr4 a in
+  if negb ((0 <=? hd 0 a) && (hd 0 a <? 2 ^ 64)) then nil else
+  if negb ((0 <=? hd 0 (tl a)) && (hd 0 (tl a) <? 2 ^ 64)) then nil else
+  dlet a := two_steps_of_p256_montgomery_reduction a in
+  if negb ((0 <=? hd 0 a) && (hd 0 a <? 2 ^ 64)) then nil else
+  if negb ((0 <=? hd 0 (tl a)) && (hd 0 (tl a) <? 2 ^ 64)) then nil else
+  dlet a := two_steps_of_p256_montgomery_reduction a in
+  if negb (eval a <? (weight bound (Nat.max (Datatypes.length a) (Datatypes.length (encode bound 4 p256))))) then nil else
+  dlet a := condsub bound a (encode bound 4 p256) in
+  if negb (4 <=? Z.of_nat (Datatypes.length a)) then nil else
+  if negb (isbounded bound a) then nil else
+  dlet a := firstn 4 a in
+  a.
+
+Lemma p256_sqr'_correct x : p256_sqr x <> nil -> p256_sqr' x = p256_sqr x.
+Proof. cbv [p256_sqr p256_sqr' Let_In]; break_match; congruence. Qed.
+
 Lemma two_steps_of_p256_montgomery_reduction_correct xs :
-  let z := eval bound (two_steps_of_p256_montgomery_reduction xs) in
-  2^128 * z mod p256 = eval bound xs mod p256 /\ (
-    0 <= eval bound xs -> 0 <= hd 0 xs < 2^64 -> 0 <= hd 0 (tl xs) < 2^64  ->
-    (eval bound xs <= ( p256+2^129-2^97)*(2^128-1) -> 0 <= z <  p256 + p256) /\
-    (eval bound xs <= (2^256+2^129-2^96)*(2^128-1) -> 0 <= z < 2^256 + p256) /\
-    (eval bound xs <= (2^256-2^223)*(2^256-2^223) -> 0 <= z < 2^128 * p256)).
+  let z := eval (two_steps_of_p256_montgomery_reduction xs) in
+  2^128 * z mod p256 = eval xs mod p256 /\ (
+    0 <= eval xs -> 0 <= hd 0 xs < 2^64 -> 0 <= hd 0 (tl xs) < 2^64  ->
+    (eval xs <= ( p256+2^129-2^97)*(2^128-1) -> 0 <= z <  p256 + p256) /\
+    (eval xs <= (2^256+2^129-2^96)*(2^128-1) -> 0 <= z < 2^256 + p256) /\
+    (eval xs <= (2^256-2^223)*(2^256-2^223) -> 0 <= z < 2^128 * p256)).
 Proof.
   cbv [Let_In two_steps_of_p256_montgomery_reduction].
   pose proof eval_hd_tl bound xs; pose proof eval_hd_tl bound (tl xs).
@@ -41,9 +115,9 @@ Proof.
   rewrite Z.add_with_get_carry_full_correct in Ex'; symmetry in Ex'; Prod.inversion_pair; rewrite ?Z.add_0_l in *.
   rewrite eval_product_scan_.
   set (_ + _) as z.
-  assert (2 ^ 128 * z = eval bound xs + (x + 2 ^ 64 * x') * p256) as Hz; [|clearbody z].
+  assert (2 ^ 128 * z = eval xs + (x + 2 ^ 64 * x') * p256) as Hz; [|clearbody z].
   { subst z.
-    enough (eval bound (map _ _) = 2^32 * x' + 2^64 * p3 * x + 2^128 * p3*x') as ->.
+    enough (eval (map _ _) = 2^32 * x' + 2^64 * p3 * x + 2^128 * p3*x') as ->.
     { cbv [p256 p3]; Z.div_mod_to_equations; nia. }
     rewrite map_app, map_repeat, eval_app, eval_repeat_0.
     cbn [List.length List.map uncurry eval PreExtra.list_rect_fbb_b list_rect].
@@ -58,183 +132,62 @@ Proof.
   lia.
 Qed.
 
-Definition p256_mul' x y :=
-  dlet xlo := firstn 2 x in
-  dlet xhi := skipn 2 x in
-  dlet a := mul bound (firstn 2 x) y in
-  dlet a := two_steps_of_p256_montgomery_reduction a in
-  dlet a := add_mul bound a xhi y in
-  dlet a := two_steps_of_p256_montgomery_reduction a in
-  dlet a := condsub bound a (encode bound 4 p256) in
-  firstn 4 a.
-
-Definition p256_mul x y :=
-  if negb ((0 <=? eval bound x) && (eval bound x <? 2^256)) then nil else
-  if negb ((0 <=? eval bound y) && (eval bound y <? 2^256)) then nil else
-  dlet xlo := firstn 2 x in
-  dlet xhi := skipn 2 x in
-  if negb ((0 <=? eval bound xlo) && (eval bound xlo <? 2^128)) then nil else
-  dlet a := mul bound (firstn 2 x) y in
-  if negb ((0 <=? hd 0 a) && (hd 0 a <? 2 ^ 64)) then nil else
-  if negb ((0 <=? hd 0 (tl a)) && (hd 0 (tl a) <? 2 ^ 64)) then nil else
-  dlet a := two_steps_of_p256_montgomery_reduction a in
-  if negb ((0 <=? eval bound xhi) && (eval bound xhi <? 2^128)) then nil else
-  dlet a := add_mul bound a xhi y in
-  if negb ((0 <=? hd 0 a) && (hd 0 a <? 2 ^ 64)) then nil else
-  if negb ((0 <=? hd 0 (tl a)) && (hd 0 (tl a) <? 2 ^ 64)) then nil else
-  dlet a := two_steps_of_p256_montgomery_reduction a in
-  if negb (eval bound a <? (weight bound (Nat.max (Datatypes.length a) (Datatypes.length (encode bound 4 p256))))) then nil else
-  dlet a := condsub bound a (encode bound 4 p256) in
-  if negb (4 <=? Z.of_nat (Datatypes.length a)) then nil else
-  if negb (isbounded bound a) then nil else
-  firstn 4 a.
-
-(*
-Require Import Coq.ZArith.ZArith.
-Require Import Coq.QArith.QArith.
-Require Import Coq.QArith.Qround.
-Require Import Coq.Strings.String.
-Require Import Coq.derive.Derive.
-Require Import Coq.Lists.List.
-Require Import Crypto.Util.LetIn.
-Require Import Crypto.Util.ZRange.
-Require Import Crypto.Util.ZUtil.Zselect.
-Require Import Crypto.Util.ZUtil.Definitions.
-Require Import Crypto.Arithmetic.Core.
-Require Import Crypto.Arithmetic.WeightStream.
-Require Crypto.PushButtonSynthesis.Primitives.
-Require Crypto.Stringification.C.
-Require Import Crypto.BoundsPipeline.
-Require Import Crypto.Util.DebugMonad.
-Require Import Crypto.Util.ZUtil.ModInv.
-
-Require Import Crypto.Util.Notations.
-Local Open Scope string_scope.
-Local Open Scope list_scope.
-Import ListNotations. Local Open Scope Z_scope.
-
-Import
-  AbstractInterpretation.Compilers
-  Language.Compilers
-  Language.API.Compilers.
-
-Import Language.API.Compilers.API.
-
-Import Associational Positional.
-
-Local Existing Instance default_translate_to_fancy.
-Local Existing Instances
-      Primitives.Options.default_PipelineOptions
-      Primitives.Options.default_PipelineToStringOptions
-      Primitives.Options.default_SynthesisOptions
-| 100.
-Local Instance : unfold_value_barrier_opt := true.
-
-Module debugging_scheduled_saturated_arithmetic.
-  Section __.
-    Import Stringification.C.
-    Import Stringification.C.Compilers.
-    Import Stringification.C.Compilers.ToString.
-
-    (* We split these off to make things a bit easier on typeclass resolution and speed things up. *)
-    Local Existing Instances ToString.C.OutputCAPI Pipeline.show_ErrorMessage.
-    Local Instance : only_signed_opt := false.
-    Local Instance : no_select_opt := false.
-    Local Instance : static_opt := true.
-    Local Instance : internal_static_opt := true.
-    Local Instance : inline_opt := true.
-    Local Instance : inline_internal_opt := true.
-    Local Instance : use_mul_for_cmovznz_opt := false.
-    Local Instance : emit_primitives_opt := true.
-    Local Instance : should_split_mul_opt := false.
-    Local Instance : should_split_multiret_opt := false.
-    Local Instance : widen_carry_opt := false.
-    Local Instance : widen_bytes_opt := true. (* true, because we don't allow byte-sized things anyway, so we should not expect carries to be widened to byte-size when emitting C code *)
-
-    (** ======= these are the changable parameters ====== *)
-    Let machine_wordsize := 64.
-    (** ================================================= *)
-    Let possible_values := prefix_with_carry [machine_wordsize].
-    Local Instance : machine_wordsize_opt := machine_wordsize. (* for show *)
-    Local Instance : no_select_size_opt := no_select_size_of_no_select machine_wordsize.
-    Local Instance : split_mul_to_opt := split_mul_to_of_should_split_mul machine_wordsize possible_values.
-    Local Instance : split_multiret_to_opt := split_multiret_to_of_should_split_multiret machine_wordsize possible_values.
-
-    Let n : nat := 4.
-    Let boundsn : list (ZRange.type.option.interp base.type.Z) := repeat (Some r[0 ~> (2^machine_wordsize - 1)]%zrange) n.
-
-    Import IdentifiersBasicGENERATED.Compilers.
-    Import API.Compilers.
-    Import APINotations.Compilers.
-
-    Import WeightStream.Saturated.
-
-Time Redirect "log"
-     Compute
-     let e :=
-       (ltac:(
-       let e := constr:(p256_mul) in
-       let e := eval cbv delta [two_steps_of_p256_montgomery_reduction p256_mul mul add_mul add_mul_limb_ product_scan product_scan_ stream.map weight stream.prefixes stream.firstn condsub] in e in
-       let r := Reify e in
-       exact r))
-                in
-     Show.show (* [show] for pretty-printing of the AST without needing lots of imports *)
-     (
-     Pipeline.BoundsPipelineToString
-        "fiat_" "p256_mul"
-        false (* subst01 *)
-        false (* inline *)
-        possible_values
-        machine_wordsize
-        e
-               (fun _ _ => []) (* comment *)
-               (Some boundsn, (Some boundsn, tt))
-               (Some boundsn)
-               (None, (None, tt))
-               (None)
-      : Pipeline.ErrorT _).
-*)
-
 Ltac lift_let :=
   match goal with
   | |- context G [let x := ?v in @?C x] =>
       let x := fresh x in
-      set v as x;
+      pose v as x;
       let g' := context G [C x] in
       let g' := eval cbv beta in g' in
       change g'
   | d := context G [let x := ?v in @?C x] |- _ =>
       let x := fresh x in
-      set v as x;
+      pose v as x;
       let g' := context G [C x] in
       let g' := eval cbv beta in g' in
       change g' in (value of d)
   | H: context G [let x := ?v in @?C x] |- _ =>
       let x := fresh x in
-      set v as x;
+      pose v as x;
       let g' := context G [C x] in
       let g' := eval cbv beta in g' in
       change g' in H
   end.
 
-Require Import AdmitAxiom.
-Lemma p256_mul_correct x y
-  (Hy : 0 <= eval bound y < p256)
-  (Hlx : (2 <= length x)%nat)
-  (z := p256_mul x y)
-  (Hcompiles : z <> nil) :
-  2^256 * eval bound z mod p256 = eval bound x * eval bound y mod p256 /\
-  (0 <= eval bound x < p256 -> 0 <= eval bound z < p256).
+Lemma eval_sqr4 xs : length xs = 4%nat -> 0 <= eval xs < 2^256 ->
+  eval (sqr4 xs) = eval xs * eval xs.
 Proof.
-  pose proof firstn_skipn 2 x as H; eapply (f_equal (eval bound)) in H.
-  rewrite eval_app, firstn_length_le in H by trivial.
+  intros H **. do 5 (destruct xs; try inversion H).
+  cbv beta delta [sqr4 Let_In].
+  repeat lift_let.
+  cbv in x0, x1, x2, x3; subst x0 x1 x2 x3.
+  subst y2.
+  rewrite add_correct; cbn [fst]. change (Nat.max _ _) with 8%nat.
+  rewrite Z.add_0_l, (eval_diagonal (Z.to_pos (2^64))).
+  subst y1.
+  rewrite eval_encode, eval_add_, Z.add_0_l, Z.add_diag.
+  subst y0 y.
+  rewrite eval_product_scan_, eval_product_scan_, ?eval_nil, ?Z.add_0_l.
+  cbn [map uncurry]; rewrite ?Z.mul_0_l, ?Z.add_0_r.
+  rewrite ?eval_cons, ?eval_nil in *;
+  progress repeat change (stream.tl ?b) with b in *;
+  progress repeat change (Z.pos (stream.hd bound)) with (2^64) in *;
+  progress repeat change (stream.hd ?b) with (b O) in *; cbv beta in *.
+  change (Z.pos (weight bound 8)) with (2^512) in *.
+  rewrite Z.mod_small; nia.
+Qed.
+
+Lemma eval_p256_mul x y (z := p256_mul x y) (Hcompiles : z <> nil) :
+  0 <= eval y < p256 ->
+  2^256 * eval z mod p256 = eval x * eval y mod p256 /\
+  (0 <= eval x < p256 -> 0 <= eval z < p256).
+Proof.
+  intros Hy.
+  pose proof firstn_skipn 2 x as H; eapply (f_equal eval) in H.
 
   cbv beta delta [p256_mul Let_In] in *.
   set (skipn 2 x) as xhi in *.
   set (firstn 2 x) as xlo in *.
-  change (stream.skipn 2 bound) with bound in *.
-  change (Z.pos (weight bound 2)) with (2^128) in *.
-
   lift_let. lift_let.
   subst y0. subst y1.
   repeat lift_let.
@@ -242,12 +195,12 @@ Proof.
   repeat match goal with
          | x := ?v |- _ =>
              let H := fresh "H" x in
-             pose proof eq_refl x : x = v as H;
+             assert (x = v) as H by reflexivity;
              move H before x;
              clearbody x
          end.
 
-  eapply (f_equal (eval bound)) in Hy0.
+  eapply (f_equal eval) in Hy0.
   rewrite (eval_mul (Z.to_pos (2^64))) in Hy0.
   change (fun _ => _) with bound in *.
   
@@ -257,6 +210,12 @@ Proof.
   end.
   rewrite Bool.negb_false_iff, Bool.andb_true_iff, Z.leb_le, Z.ltb_lt in *.
 
+  rewrite eval_app in H.
+  rewrite 2Hxlo in H at 2.
+  rewrite !firstn_length_le in H by lia.
+  progress change (Z.pos (weight bound 2)) with (2^128) in *.
+  progress change (stream.skipn _ bound) with bound in *.
+
   pose proof two_steps_of_p256_montgomery_reduction_correct y0 as HH.
   rewrite <-Hy1, Hy0 in HH; clear Hy1; cbv zeta in HH; case HH as [Hy1 HH'1].
 
@@ -264,7 +223,7 @@ Proof.
   apply proj1 in HH'1.
   do 1 specialize (HH'1 ltac:(cbv [p256] in *; nia)).
 
-  eapply (f_equal (eval bound)) in Hy2.
+  eapply (f_equal eval) in Hy2.
   rewrite (eval_add_mul (Z.to_pos (2^64))) in Hy2.
   change (fun _ => _) with bound in *.
 
@@ -272,14 +231,14 @@ Proof.
   pose proof Hy3 as Hy3'.
   rewrite <-Hy3, Hy2 in HH; clear Hy3; cbv zeta in HH; case HH as [Hy3 HH'2].
 
-  assert (HH : (2 ^ 256 * eval bound y3) mod p256 =
-    ((2^128 * eval bound y1) mod p256 + 2^128 * eval bound xhi * eval bound y) mod p256).
+  assert (HH : (2 ^ 256 * eval y3) mod p256 =
+    ((2^128 * eval y1) mod p256 + 2^128 * eval xhi * eval y) mod p256).
   { clear -Hy3; cbv [p256] in *; Z.div_mod_to_equations; nia. }
   rewrite Hy1 in HH; clear Hy1 Hy3; autorewrite with pull_Zmod in HH.
-  replace (eval bound xlo * eval bound y + 2 ^ 128 * eval bound xhi * eval bound y)
-    with (eval bound x * eval bound y) in HH by nia.
+  replace (eval xlo * eval y + 2 ^ 128 * eval xhi * eval y)
+    with (eval x * eval y) in HH by nia.
 
-  eapply (f_equal (eval bound)) in Hy4.
+  eapply (f_equal eval) in Hy4.
   rewrite eval_condsub, eval_encode, Z.mod_small in Hy4.
   2: { cbv. intuition congruence. }
   2: { trivial. }
@@ -288,123 +247,28 @@ Proof.
 
   do 3 specialize (HH'2 ltac:(cbv [p256] in *; nia)).
 
-  eapply (f_equal (eval bound)) in Hz.
-  rewrite <-e, eval_firstn_encode in Hz.
-  2: { lia. }
-  change (Z.pos (weight bound 4)) with (2^256) in *.
-  rewrite Z.mod_small in Hz.
-  2: {
-    apply proj2, proj1 in HH'2.
+  eapply (f_equal eval) in Hz.
+  rewrite <-e, eval_firstn_encode in Hz by lia.
+  progress change (Z.pos (weight bound 4)) with (2^256) in *.
+  rewrite Z.mod_small in Hz; cycle 1.
+  { apply proj2, proj1 in HH'2.
     do 1 specialize (HH'2 ltac:(cbv [p256] in *; nia)).
-    destruct (Z.leb_spec p256 (eval bound y3)) in *; simpl Z.b2z in *; cbv [p256] in *; lia. }
+    destruct (Z.leb_spec p256 (eval y3)) in *; simpl Z.b2z in *; cbv [p256] in *; lia. }
 
   rewrite Hz, Hy4.
   split.
-  { Modulo.push_Zmod; Modulo.pull_Zmod.
-    rewrite Z.mul_0_r, Z.sub_0_r; trivial. }
-
-  intros.
-  destruct (Z.leb_spec p256 (eval bound y3)) in *; simpl Z.b2z in *; cbv [p256] in *; nia.
+  { Modulo.push_Zmod; Modulo.pull_Zmod. rewrite Z.mul_0_r, Z.sub_0_r; trivial. }
+  { intros. destruct (Z.leb_spec p256 (eval y3)) in *; simpl Z.b2z in *; cbv [p256] in *; nia. }
 Qed.
 
-(*
-Print Assumptions p256_mul_correct.
-Closed under the global context
-*)
+Lemma p256_sqr_sufficient_bound : p256 < 2^256-2^223. Proof. compute. trivial. Qed.
 
-Definition diagonal b (pps : list (Z * Z)) :=
-  flat_map (fun '(x, y) =>
-    let '(lo, hi) := Z.mul_split b x y in
-    [lo; hi]
-  ) pps.
-
-Lemma eval_diagonal (b : positive) pps :
-  eval (fun _ => b) (diagonal b pps) =
-  eval (fun _ => Pos.mul b b) (map (uncurry Z.mul) pps).
+Lemma eval_p256_sqr x (z := p256_sqr x) (Hcompiles : z <> nil) :
+  0 <= eval x < 2^256-2^223 ->
+  2^256 * eval z mod p256 = eval x * eval x mod p256 /\
+  0 <= eval z < p256.
 Proof.
-  induction pps as [|[x y] ]; [trivial|].
-  cbn [diagonal flat_map map fst snd uncurry].
-  progress change (flat_map _ ?xs) with (diagonal (Z.pos b) xs).
-  rewrite Z.mul_split_correct.
-  cbn [app]; rewrite ?eval_cons, ?eval_nil; cbn [length].
-  progress repeat change (stream.tl ?b) with b.
-  progress repeat change (stream.hd ?b) with (b O); cbv beta.
-  Z.div_mod_to_equations; nia.
-Qed.
-
-Definition sqr4 xs : list Z :=
-  let x0 := nth_default 0 xs 0 in
-  let x1 := nth_default 0 xs 1 in
-  let x2 := nth_default 0 xs 2 in
-  let x3 := nth_default 0 xs 3 in
-  dlet acc := product_scan_ bound [] [(0,0); (0,0); (0, 0); (x1, x2)] 0 0 0 in
-  dlet acc := product_scan_ bound acc [(0, 0); (x0, x1); (x0, x2); (x0, x3); (x1, x3); (x2, x3)] 0 0 0 in
-  dlet acc := add_ bound 0 acc acc in
-  dlet acc := fst (add bound 0 acc (diagonal (2^64) [(x0,x0); (x1, x1); (x2, x2); (x3, x3)]))
-  in acc.
-
-Lemma eval_sqr4' x0 x1 x2 x3 (xs:=[x0;x1;x2;x3]) :
-  0 <= eval bound xs < 2^256 -> eval bound (sqr4 xs) = eval bound xs * eval bound xs.
-Proof.
-  cbv beta delta [sqr4 Let_In].
-  repeat (progress change (?f (let x := ?v in @?C x) = ?R) with (let x := v in f (C x) = R); cbv beta; intros).
-  cbv in x, x4, x5, x6; subst x x4 x5 x6.
-  subst x10.
-  rewrite add_correct; cbn [fst]. change (Nat.max _ _) with 8%nat.
-  rewrite Z.add_0_l, (eval_diagonal (Z.to_pos (2^64))).
-  subst x9.
-  rewrite eval_encode, eval_add_, Z.add_0_l, Z.add_diag.
-  subst x8.
-  rewrite eval_product_scan_.
-  subst x7.
-  rewrite eval_product_scan_, ?eval_nil, ?Z.add_0_l.
-  cbn [map uncurry]; rewrite ?Z.mul_0_l, ?Z.add_0_r.
-  subst xs.
-  rewrite ?eval_cons, ?eval_nil in *;
-  progress repeat change (stream.tl ?b) with b in *;
-  progress repeat change (Z.pos (stream.hd bound)) with (2^64) in *;
-  progress repeat change (stream.hd ?b) with (b O) in *; cbv beta in *.
-  change (Z.pos (weight bound 8)) with (2^512) in *.
-  rewrite Z.mod_small; nia.
-Qed.
-
-Lemma eval_sqr4 xs :
-  length xs = 4%nat ->
-  0 <= eval bound xs < 2 ^ 256 ->
-  eval bound (sqr4 xs) = eval bound xs * eval bound xs.
-Proof. intros H *. do 5 (destruct xs; try inversion H). apply eval_sqr4'. Qed.
-
-Definition p256_sqr' a :=
-  dlet a := sqr4 a in
-  dlet a := two_steps_of_p256_montgomery_reduction a in
-  dlet a := two_steps_of_p256_montgomery_reduction a in
-  dlet a := condsub bound a (encode bound 4 p256) in
-  dlet a := firstn 4 a in
-  a.
-
-Definition p256_sqr a :=
-  if negb (4 =? Z.of_nat (Datatypes.length a)) then nil else
-  dlet a := sqr4 a in
-  if negb ((0 <=? hd 0 a) && (hd 0 a <? 2 ^ 64)) then nil else
-  if negb ((0 <=? hd 0 (tl a)) && (hd 0 (tl a) <? 2 ^ 64)) then nil else
-  dlet a := two_steps_of_p256_montgomery_reduction a in
-  if negb ((0 <=? hd 0 a) && (hd 0 a <? 2 ^ 64)) then nil else
-  if negb ((0 <=? hd 0 (tl a)) && (hd 0 (tl a) <? 2 ^ 64)) then nil else
-  dlet a := two_steps_of_p256_montgomery_reduction a in
-  if negb (eval bound a <? (weight bound (Nat.max (Datatypes.length a) (Datatypes.length (encode bound 4 p256))))) then nil else
-  dlet a := condsub bound a (encode bound 4 p256) in
-  if negb (4 <=? Z.of_nat (Datatypes.length a)) then nil else
-  if negb (isbounded bound a) then nil else
-  dlet a := firstn 4 a in
-  a.
-
-Lemma p256_sqr_correct x
-  (Hy : 0 <= eval bound x (* < p256*) < 2^256-2^223 )
-  (z := p256_sqr x)
-  (Hcompiles : z <> nil) :
-  2^256 * eval bound z mod p256 = eval bound x * eval bound x mod p256 /\
-  0 <= eval bound z < p256.
-Proof.
+  intros Hy.
   cbv beta delta [p256_sqr Let_In] in *.
   repeat lift_let.
 
@@ -424,7 +288,7 @@ Proof.
 
   rewrite Bool.negb_false_iff, Bool.andb_true_iff, Z.leb_le, Z.ltb_lt in *.
 
-  eapply (f_equal (eval bound)) in Hy0.
+  eapply (f_equal eval) in Hy0.
   rewrite eval_sqr4 in Hy0 by (cbv [p256] in *; lia).
 
   pose proof two_steps_of_p256_montgomery_reduction_correct y as HH.
@@ -441,7 +305,7 @@ Proof.
   apply proj1 in HH'2.
   do 1 specialize (HH'2 ltac:(cbv [p256] in *; nia)).
 
-  eapply (f_equal (eval bound)) in Hy3.
+  eapply (f_equal eval) in Hy3.
   rewrite eval_condsub, eval_encode, Z.mod_small in Hy3.
   2: { cbv. intuition congruence. }
   2: { trivial. }
@@ -449,19 +313,19 @@ Proof.
   destruct (isbounded_correct bound y2) in *; [|discriminate].
 
   subst y3.
-  eapply (f_equal (eval bound)) in Hz.
+  eapply (f_equal eval) in Hz.
   rewrite <-e, eval_firstn_encode in Hz.
   2: { lia. }
   change (Z.pos (weight bound 4)) with (2^256) in *.
   rewrite Z.mod_small in Hz.
-  2: { destruct (Z.leb_spec p256 (eval bound y1)) in *; simpl Z.b2z in *; cbv [p256] in *; lia. }
+  2: { destruct (Z.leb_spec p256 (eval y1)) in *; simpl Z.b2z in *; cbv [p256] in *; lia. }
 
   rewrite Hz, Hy3.
   split.
   { Modulo.push_Zmod; Modulo.pull_Zmod.
     rewrite Z.mul_0_r, Z.sub_0_r.
-    replace (2 ^ 256 * eval bound y1)
-    with (2 ^ 128 * (2 ^ 128 * eval bound y1)) by lia.
+    replace (2 ^ 256 * eval y1)
+    with (2 ^ 128 * (2 ^ 128 * eval y1)) by lia.
     rewrite <-Z.mul_mod_idemp_r by (cbv; lia).
     rewrite Hy2.
     rewrite Z.mul_mod_idemp_r by (cbv; lia).
@@ -469,5 +333,5 @@ Proof.
   }
 
   intros.
-  destruct (Z.leb_spec p256 (eval bound y1)) in *; simpl Z.b2z in *; cbv [p256] in *; nia.
+  destruct (Z.leb_spec p256 (eval y1)) in *; simpl Z.b2z in *; cbv [p256] in *; nia.
 Qed.
