src/PushButtonSynthesis/P256ADXReificationCache.v
@@ -9,9 +9,6 @@ Import Basic.GallinaAndReifiedIdentList IdentifiersBasicGENERATED.Compilers.
 Import Coq.ZArith.ZArith.
 Import Coq.derive.Derive.
 Import Crypto.PushButtonSynthesis.ReificationCache.
-Import
-  Language.API.Compilers
-  Language.Wf.Compilers.
 
 Derive reified_p256_mul
        SuchThat (is_reification_of reified_p256_mul p256_mul)
@@ -21,7 +18,7 @@ Proof.
   instantiate (1:=
     (ltac:(
       let e := constr:(p256_mul) in
-       let e := eval cbv delta [two_steps_of_p256_montgomery_reduction p256_mul mul add_mul add_mul_limb_ product_scan product_scan_ stream.map weight stream.prefixes stream.firstn condsub] in e in
+      let e := eval cbv delta [p256_sqr sqr4 two_steps_of_p256_montgomery_reduction p256_mul mul add_mul add_mul_limb_ product_scan product_scan_ stream.map weight stream.prefixes stream.firstn condsub] in e in
       let r := Reify e in
       exact r))
     ) in (value of reified_p256_mul).
@@ -37,7 +34,7 @@ Proof.
   instantiate (1:=
     (ltac:(
       let e := constr:(p256_sqr) in
-       let e := eval cbv delta [p256_sqr sqr4 two_steps_of_p256_montgomery_reduction p256_mul mul add_mul add_mul_limb_ product_scan product_scan_ stream.map weight stream.prefixes stream.firstn condsub] in e in
+      let e := eval cbv delta [p256_sqr sqr4 two_steps_of_p256_montgomery_reduction p256_mul mul add_mul add_mul_limb_ product_scan product_scan_ stream.map weight stream.prefixes stream.firstn condsub] in e in
       let r := Reify e in
       exact r))
     ) in (value of reified_p256_sqr).
