src/SlowPrimeSynthesisExamples.v
@@ -88,36 +88,20 @@ Module debugging_scheduled_saturated_arithmetic.
 
     Definition bound (_ : Datatypes.nat) := Z.to_pos (2^64).
 
-    (*
-    Definition mulmod (c : BinNums.Z := 38) (a b : list BinNums.Z) :=
-      let p := mul bound a b in
-      let (lo, hi) := add_mul_limb bound (firstn n p) c (skipn n p) in
-      if c * Z.abs hi <=? 2^machine_wordsize - c
-      then reduce' bound 1 c lo [hi]
-      else lo ++ [hi].
-     *)
-
-    (*
-    Ltac2 Set reify_debug_level := 1.
-    Check ltac:(
-              let e := constr:(addmod bound) in
-              let e := eval cbv delta [addmod reduce' add_mul_limb add_mul_limb' stream.map weight stream.prefixes] in e in
-              let r := Reify e in
-              exact r).
-    *)
-
-    Fail Check ltac:(
+    Goal True.
+    assert_fails (idtac;
       let e := constr:(weight (fun _ => 10)%positive 2) in
       let e := eval cbv [stream.map weight] in e in
       (* let e := eval cbv delta [stream.prefixes] in e in *)
-      idtac e;
-      let r := Reify e in exact r).
-    Check ltac:(
+      (* idtac e; *)
+      let r := Reify e in pose r).
+    assert_succeeds (idtac;
       let e := constr:(weight (fun _ => 10)%positive 2) in
       let e := eval cbv [stream.map weight] in e in
       let e := eval cbv delta [stream.prefixes] in e in
-      idtac e;
-      let r := Reify e in exact r).
+      (* idtac e; *)
+      let r := Reify e in pose r).
+    Abort.
 
     Goal True.
     pose (
@@ -185,7 +169,7 @@ Module debugging_scheduled_saturated_arithmetic.
                     let (lo, hi) := add_mul_small bound [] x ys in
                     reduce bound 1%nat 38 lo [hi]
                   ) in
-                  let e := eval cbv delta [reduce reduce' add_mul_limb product_scan stream.map weight stream.prefixes] in e in
+                  let e := eval cbv delta [reduce reduce' add_mul_small product_scan stream.map weight stream.prefixes] in e in
                   let r := Reify e in
                   exact r)
                    (fun _ _ => []) (* comment *)
@@ -206,8 +190,7 @@ Module debugging_scheduled_saturated_arithmetic.
             false (* inline *)
             possible_values
             machine_wordsize
-            ltac:(let e := constr:(canon bound (2^255-19)) in
-                  let e := eval cbv delta [n canon stream.map weight stream.prefixes] in e in
+            ltac:(let e := constr:(fun x => dlet x := x in condsubs bound 2 x (encode bound 4 (2^255-19))) in
                   let r := Reify e in
                   exact r)
                    (fun _ _ => []) (* comment *)
@@ -225,8 +208,8 @@ Module debugging_scheduled_saturated_arithmetic.
             false (* inline *)
             possible_values
             machine_wordsize
-            ltac:(let n := (eval cbv in n) (* needs to be reduced to reify correctly *) in
-                  let r := Reify (select) in
+            ltac:(let e := constr:(select) in
+                  let r := Reify e in
                   exact r)
                    (fun _ _ => []) (* comment *)
                    (Some (r[0 ~>1]%zrange), (Some boundsn, (Some boundsn, tt)))
@@ -243,12 +226,12 @@ Module debugging_scheduled_saturated_arithmetic.
             false (* inline *)
             possible_values
             machine_wordsize
-            ltac:(let n := (eval cbv in n) (* needs to be reduced to reify correctly *) in
-                  let r := Reify (cswap) in
+            ltac:(let e := constr:(cswap') in
+                  let r := Reify e in
                   exact r)
                    (fun _ _ => []) (* comment *)
                    (Some (r[0 ~>1]%zrange), (Some boundsn, (Some boundsn, tt)))
-                   (Some boundsn, Some boundsn)
+                   ((Some boundsn, Some boundsn))
                    (None, (None, (None, tt)))
                    (None, None)).
 
@@ -280,7 +263,7 @@ Module debugging_scheduled_saturated_arithmetic.
             possible_values
             machine_wordsize
             ltac:(let e := constr:(mul bound) in
-                  let e := eval cbv delta [mulmod mul add_mul add_mul_limb_ add_mul_limb reduce' product_scan stream.map weight stream.prefixes] in e in
+            let e := eval cbv delta [mulmod mul add_mul add_mul_limb_ product_scan_ add_mul_small product_scan' reduce' product_scan stream.map weight stream.prefixes] in e in
                   let r := Reify e in
                   exact r)
                    (fun _ _ => []) (* comment *)
@@ -304,7 +287,7 @@ Module debugging_scheduled_saturated_arithmetic.
             machine_wordsize
             ltac:(
                   let e := constr:(mulmod bound 4 38) in
-                  let e := eval cbv delta [mulmod mul add_mul add_mul_limb_ add_mul_limb reduce' product_scan stream.map weight stream.prefixes] in e in
+                  let e := eval cbv delta [mulmod mul add_mul add_mul_limb_ product_scan_ add_mul_small product_scan' reduce' product_scan stream.map weight stream.prefixes] in e in
                   let r := Reify e in
                   exact r)
                    (fun _ _ => []) (* comment *)
@@ -330,7 +313,7 @@ Import P256ADX.
             machine_wordsize
             ltac:(
                   let e := constr:(sqr4) in
-                  let e := eval cbv delta [sqr4 two_steps_of_p256_montgomery_friendly_reduction p256_mul mul add_mul add_mul_limb_ add_mul_limb reduce' product_scan product_scan_ stream.map weight stream.prefixes] in e in
+                  let e := eval cbv delta [sqr4 two_steps_of_p256_montgomery_reduction p256_mul mul add_mul add_mul_limb_ add_mul_limb_ reduce' product_scan product_scan_ stream.map weight stream.prefixes] in e in
                   let r := Reify e in
                   exact r)
                    (fun _ _ => []) (* comment *)
@@ -345,13 +328,13 @@ Import P256ADX.
          Show.show (* [show] for pretty-printing of the AST without needing lots of imports *)
          (
          Pipeline.BoundsPipelineToString
-            "fiat_" "p256mul2w"
+            "fiat_" "p256red2w"
             false (* subst01 *)
             false (* inline *)
             possible_values
             machine_wordsize
-            ltac:(let e := constr:(two_steps_of_p256_montgomery_friendly_reduction) in
-            let e := eval cbv delta [two_steps_of_p256_montgomery_friendly_reduction mulmod mul add_mul add_mul_limb_ add_mul_limb reduce' product_scan_ product_scan stream.map weight stream.prefixes] in e in
+            ltac:(let e := constr:(two_steps_of_p256_montgomery_reduction) in
+                  let e := eval cbv delta [p256_sqr sqr4 two_steps_of_p256_montgomery_reduction p256_mul mul add_mul add_mul_limb_ product_scan product_scan_ stream.map weight stream.prefixes stream.firstn condsub] in e in
                   let r := Reify e in
                   exact r)
                    (fun _ _ => []) (* comment *)
@@ -365,7 +348,7 @@ Import P256ADX.
   fiat_addcarryx_u64(&x3, &x4, 0x0, (arg1[1]), x1);
   fiat_mulx_u64(&x5, &x6, UINT64_C(0x100000000), x3);
   fiat_addcarryx_u64(&x7, &x8, x4, (arg1[2]), x2);
-  fiat_addcarryx_u64(&x9, &x10, 0x0, x7, x5);
+  fiat_addcarryx_u64(&x9, &x10, 0imbx0, x7, x5);
   fiat_mulx_u64(&x11, &x12, UINT64_C(0xffffffff00000001), (arg1[0]));
   fiat_addcarryx_u64(&x13, &x14, x8, (arg1[3]), x6);
   fiat_addcarryx_u64(&x15, &x16, x10, x13, x11);
@@ -393,8 +376,8 @@ Import P256ADX.
             possible_values
             machine_wordsize
             ltac:(
-                  let e := constr:(p256_mul) in
-                  let e := eval cbv delta [two_steps_of_p256_montgomery_friendly_reduction p256_mul mul add_mul add_mul_limb_ add_mul_limb reduce' product_scan product_scan_ stream.map weight stream.prefixes] in e in
+                  let e := constr:(p256_mul') in
+                  let e := eval cbv delta [p256_sqr sqr4 two_steps_of_p256_montgomery_reduction p256_mul' mul add_mul add_mul_limb_ product_scan product_scan_ stream.map weight stream.prefixes stream.firstn condsub] in e in
                   let r := Reify e in
                   exact r)
                    (fun _ _ => []) (* comment *)
@@ -403,6 +386,97 @@ Import P256ADX.
                    (None, (None, tt))
                    (None)
           : Pipeline.ErrorT _).
+(*fiat_mulx_u64(&x3, &x4, (arg1[0]), (arg2[0]));
+  fiat_mulx_u64(&x5, &x6, (arg1[0]), (arg2[1]));
+  fiat_addcarryx_u64(&x7, &x8, 0x0, x4, x5);
+  fiat_mulx_u64(&x9, &x10, (arg1[0]), (arg2[2]));
+  fiat_addcarryx_u64(&x11, &x12, x8, x6, x9);
+  fiat_mulx_u64(&x13, &x14, (arg1[0]), (arg2[3]));
+  fiat_addcarryx_u64(&x15, &x16, x12, x10, x13);
+  x17 = (x16 + x14);
+  fiat_mulx_u64(&x18, &x19, (arg1[1]), (arg2[0]));
+  fiat_addcarryx_u64(&x20, &x21, 0x0, x7, x18);
+  fiat_mulx_u64(&x22, &x23, (arg1[1]), (arg2[1]));
+  fiat_addcarryx_u64(&x24, &x25, 0x0, x11, x19);
+  fiat_addcarryx_u64(&x26, &x27, x21, x24, x22);
+  fiat_mulx_u64(&x28, &x29, (arg1[1]), (arg2[2]));
+  fiat_addcarryx_u64(&x30, &x31, x25, x15, x23);
+  fiat_addcarryx_u64(&x32, &x33, x27, x30, x28);
+  fiat_mulx_u64(&x34, &x35, (arg1[1]), (arg2[3]));
+  fiat_addcarryx_u64(&x36, &x37, x31, x17, x29);
+  fiat_addcarryx_u64(&x38, &x39, x33, x36, x34);
+  x40 = (x37 + x35);
+  fiat_addcarryx_u64(&x41, &x42, x39, x40, 0x0);
+  fiat_mulx_u64(&x43, &x44, UINT64_C(0x100000000), x3);
+  fiat_addcarryx_u64(&x45, &x46, 0x0, x20, x43);
+  fiat_mulx_u64(&x47, &x48, UINT64_C(0x100000000), x45);
+  fiat_addcarryx_u64(&x49, &x50, x46, x26, x44);
+  fiat_addcarryx_u64(&x51, &x52, 0x0, x49, x47);
+  fiat_mulx_u64(&x53, &x54, UINT64_C(0xffffffff00000001), x3);
+  fiat_addcarryx_u64(&x55, &x56, x50, x32, x48);
+  fiat_addcarryx_u64(&x57, &x58, x52, x55, x53);
+  fiat_mulx_u64(&x59, &x60, UINT64_C(0xffffffff00000001), x45);
+  fiat_addcarryx_u64(&x61, &x62, x56, x38, x54);
+  fiat_addcarryx_u64(&x63, &x64, x58, x61, x59);
+  fiat_addcarryx_u64(&x65, &x66, x62, x41, x60);
+  fiat_addcarryx_u64(&x67, &x68, x64, x65, 0x0);
+  x69 = ((uint64_t)x68 + x66);
+  fiat_mulx_u64(&x70, &x71, x1, (arg2[0]));
+  fiat_addcarryx_u64(&x72, &x73, 0x0, x51, x70);
+  fiat_mulx_u64(&x74, &x75, x1, (arg2[1]));
+  fiat_addcarryx_u64(&x76, &x77, 0x0, x57, x71);
+  fiat_addcarryx_u64(&x78, &x79, x73, x76, x74);
+  fiat_mulx_u64(&x80, &x81, x1, (arg2[2]));
+  fiat_addcarryx_u64(&x82, &x83, x77, x63, x75);
+  fiat_addcarryx_u64(&x84, &x85, x79, x82, x80);
+  fiat_mulx_u64(&x86, &x87, x1, (arg2[3]));
+  fiat_addcarryx_u64(&x88, &x89, x83, x67, x81);
+  fiat_addcarryx_u64(&x90, &x91, x85, x88, x86);
+  x92 = (x89 + x87);
+  fiat_addcarryx_u64(&x93, &x94, x91, x92, 0x0);
+  fiat_addcarryx_u64(&x95, &x96, 0x0, x69, x93);
+  fiat_mulx_u64(&x97, &x98, x2, (arg2[0]));
+  fiat_addcarryx_u64(&x99, &x100, 0x0, x78, x97);
+  fiat_mulx_u64(&x101, &x102, x2, (arg2[1]));
+  fiat_addcarryx_u64(&x103, &x104, 0x0, x84, x98);
+  fiat_addcarryx_u64(&x105, &x106, x100, x103, x101);
+  fiat_mulx_u64(&x107, &x108, x2, (arg2[2]));
+  fiat_addcarryx_u64(&x109, &x110, x104, x90, x102);
+  fiat_addcarryx_u64(&x111, &x112, x106, x109, x107);
+  fiat_mulx_u64(&x113, &x114, x2, (arg2[3]));
+  fiat_addcarryx_u64(&x115, &x116, x110, x95, x108);
+  fiat_addcarryx_u64(&x117, &x118, x112, x115, x113);
+  x119 = (x116 + x114);
+  fiat_addcarryx_u64(&x120, &x121, x118, x119, 0x0);
+  fiat_addcarryx_u64(&x122, &x123, 0x0, x96, x120);
+  fiat_mulx_u64(&x124, &x125, UINT64_C(0x100000000), x72);
+  fiat_addcarryx_u64(&x126, &x127, 0x0, x99, x124);
+  fiat_mulx_u64(&x128, &x129, UINT64_C(0x100000000), x126);
+  fiat_addcarryx_u64(&x130, &x131, x127, x105, x125);
+  fiat_addcarryx_u64(&x132, &x133, 0x0, x130, x128);
+  fiat_mulx_u64(&x134, &x135, UINT64_C(0xffffffff00000001), x72);
+  fiat_addcarryx_u64(&x136, &x137, x131, x111, x129);
+  fiat_addcarryx_u64(&x138, &x139, x133, x136, x134);
+  fiat_mulx_u64(&x140, &x141, UINT64_C(0xffffffff00000001), x126);
+  fiat_addcarryx_u64(&x142, &x143, x137, x117, x135);
+  fiat_addcarryx_u64(&x144, &x145, x139, x142, x140);
+  fiat_addcarryx_u64(&x146, &x147, x143, x122, x141);
+  fiat_addcarryx_u64(&x148, &x149, x145, x146, 0x0);
+  x150 = ((uint64_t)x147 + x123);
+  x151 = (x149 + x150);
+  fiat_subborrowx_u64(&x152, &x153, 0x0, x132, UINT64_C(0xffffffffffffffff));
+  fiat_subborrowx_u64(&x154, &x155, x153, x138, UINT32_C(0xffffffff));
+  fiat_subborrowx_u64(&x156, &x157, x155, x144, 0x0);
+  fiat_subborrowx_u64(&x158, &x159, x157, x148, UINT64_C(0xffffffff00000001));
+  fiat_subborrowx_u64(&x160, &x161, x159, x151, 0x0);
+  fiat_cmovznz_u64(&x162, x161, x152, x132);
+  fiat_cmovznz_u64(&x163, x161, x154, x138);
+  fiat_cmovznz_u64(&x164, x161, x156, x144);
+  fiat_cmovznz_u64(&x165, x161, x158, x148);
+  out1[0] = x162;
+  out1[1] = x163;
+  out1[2] = x164;
+  out1[3] = x165; *)
 
     (*
     Require Stringification.JSON.
@@ -419,8 +493,8 @@ Import P256ADX.
             possible_values
             machine_wordsize
             ltac:(
-                  let e := constr:(p256_sqr) in
-                  let e := eval cbv delta [p256_sqr sqr4 two_steps_of_p256_montgomery_friendly_reduction p256_mul mul add_mul add_mul_limb_ add_mul_limb reduce' product_scan product_scan_ stream.map weight stream.prefixes] in e in
+                  let e := constr:(p256_sqr') in
+                  let e := eval cbv delta [p256_sqr' sqr4 two_steps_of_p256_montgomery_reduction p256_mul mul add_mul add_mul_limb_ product_scan product_scan_ stream.map weight stream.prefixes stream.firstn condsub] in e in
                   let r := Reify e in
                   exact r)
                    (fun _ _ => []) (* comment *)
@@ -433,6 +507,83 @@ Import P256ADX.
         ) in
       let t := eval vm_compute in t in
       print_string t.
+(*fiat_mulx_u64(&x1, &x2, (arg1[1]), (arg1[2]));
+  fiat_mulx_u64(&x3, &x4, (arg1[0]), (arg1[1]));
+  fiat_mulx_u64(&x5, &x6, (arg1[0]), (arg1[2]));
+  fiat_addcarryx_u64(&x7, &x8, 0x0, x4, x5);
+  fiat_mulx_u64(&x9, &x10, (arg1[0]), (arg1[3]));
+  fiat_addcarryx_u64(&x11, &x12, 0x0, x1, x6);
+  fiat_addcarryx_u64(&x13, &x14, x8, x11, x9);
+  fiat_mulx_u64(&x15, &x16, (arg1[1]), (arg1[3]));
+  fiat_addcarryx_u64(&x17, &x18, x12, x2, x10);
+  fiat_addcarryx_u64(&x19, &x20, x14, x17, x15);
+  fiat_mulx_u64(&x21, &x22, (arg1[2]), (arg1[3]));
+  x23 = (x18 + x16);
+  fiat_addcarryx_u64(&x24, &x25, x20, x23, x21);
+  x26 = (x25 + x22);
+  fiat_addcarryx_u64(&x27, &x28, 0x0, x3, x3);
+  fiat_addcarryx_u64(&x29, &x30, x28, x7, x7);
+  fiat_addcarryx_u64(&x31, &x32, x30, x13, x13);
+  fiat_addcarryx_u64(&x33, &x34, x32, x19, x19);
+  fiat_addcarryx_u64(&x35, &x36, x34, x24, x24);
+  fiat_addcarryx_u64(&x37, &x38, x36, x26, x26);
+  fiat_mulx_u64(&x39, &x40, (arg1[3]), (arg1[3]));
+  fiat_mulx_u64(&x41, &x42, (arg1[2]), (arg1[2]));
+  fiat_mulx_u64(&x43, &x44, (arg1[1]), (arg1[1]));
+  fiat_mulx_u64(&x45, &x46, (arg1[0]), (arg1[0]));
+  fiat_addcarryx_u64(&x47, &x48, 0x0, x27, x46);
+  fiat_addcarryx_u64(&x49, &x50, x48, x29, x43);
+  fiat_addcarryx_u64(&x51, &x52, x50, x31, x44);
+  fiat_addcarryx_u64(&x53, &x54, x52, x33, x41);
+  fiat_addcarryx_u64(&x55, &x56, x54, x35, x42);
+  fiat_addcarryx_u64(&x57, &x58, x56, x37, x39);
+  fiat_addcarryx_u64(&x59, &x60, x58, x38, x40);
+  fiat_mulx_u64(&x61, &x62, UINT64_C(0x100000000), x45);
+  fiat_addcarryx_u64(&x63, &x64, 0x0, x47, x61);
+  fiat_mulx_u64(&x65, &x66, UINT64_C(0x100000000), x63);
+  fiat_addcarryx_u64(&x67, &x68, x64, x49, x62);
+  fiat_addcarryx_u64(&x69, &x70, 0x0, x67, x65);
+  fiat_mulx_u64(&x71, &x72, UINT64_C(0xffffffff00000001), x45);
+  fiat_addcarryx_u64(&x73, &x74, x68, x51, x66);
+  fiat_addcarryx_u64(&x75, &x76, x70, x73, x71);
+  fiat_mulx_u64(&x77, &x78, UINT64_C(0xffffffff00000001), x63);
+  fiat_addcarryx_u64(&x79, &x80, x74, x53, x72);
+  fiat_addcarryx_u64(&x81, &x82, x76, x79, x77);
+  fiat_addcarryx_u64(&x83, &x84, x80, x55, x78);
+  fiat_addcarryx_u64(&x85, &x86, x82, x83, 0x0);
+  fiat_addcarryx_u64(&x87, &x88, x84, x57, 0x0);
+  fiat_addcarryx_u64(&x89, &x90, x86, x87, 0x0);
+  fiat_addcarryx_u64(&x91, &x92, x88, x59, 0x0);
+  fiat_addcarryx_u64(&x93, &x94, x90, x91, 0x0);
+  x95 = ((uint64_t)x94 + x92);
+  fiat_mulx_u64(&x96, &x97, UINT64_C(0x100000000), x69);
+  fiat_addcarryx_u64(&x98, &x99, 0x0, x75, x96);
+  fiat_mulx_u64(&x100, &x101, UINT64_C(0x100000000), x98);
+  fiat_addcarryx_u64(&x102, &x103, x99, x81, x97);
+  fiat_addcarryx_u64(&x104, &x105, 0x0, x102, x100);
+  fiat_mulx_u64(&x106, &x107, UINT64_C(0xffffffff00000001), x69);
+  fiat_addcarryx_u64(&x108, &x109, x103, x85, x101);
+  fiat_addcarryx_u64(&x110, &x111, x105, x108, x106);
+  fiat_mulx_u64(&x112, &x113, UINT64_C(0xffffffff00000001), x98);
+  fiat_addcarryx_u64(&x114, &x115, x109, x89, x107);
+  fiat_addcarryx_u64(&x116, &x117, x111, x114, x112);
+  fiat_addcarryx_u64(&x118, &x119, x115, x93, x113);
+  fiat_addcarryx_u64(&x120, &x121, x117, x118, 0x0);
+  x122 = (x119 + x95);
+  x123 = (x121 + x122);
+  fiat_subborrowx_u64(&x124, &x125, 0x0, x104, UINT64_C(0xffffffffffffffff));
+  fiat_subborrowx_u64(&x126, &x127, x125, x110, UINT32_C(0xffffffff));
+  fiat_subborrowx_u64(&x128, &x129, x127, x116, 0x0);
+  fiat_subborrowx_u64(&x130, &x131, x129, x120, UINT64_C(0xffffffff00000001));
+  fiat_subborrowx_u64(&x132, &x133, x131, x123, 0x0);
+  fiat_cmovznz_u64(&x134, x133, x124, x104);
+  fiat_cmovznz_u64(&x135, x133, x126, x110);
+  fiat_cmovznz_u64(&x136, x133, x128, x116);
+  fiat_cmovznz_u64(&x137, x133, x130, x120);
+  out1[0] = x134;
+  out1[1] = x135;
+  out1[2] = x136;
+   out1[3] = x137;*)
     Abort.
 
 
